WIP on 19

HumanEvalLean/HumanEval19.lean
@@ -1,7 +1,92 @@
 module
 
-def sort_numbers : Unit :=
-  ()
+import Std.Data.TreeMap.Lemmas
+import Std.Data.Iterators.Producers.Array
+import Std.Data.Iterators.Producers.Range
+import Std.Data.Iterators.Lemmas.Producers.Range
+
+def numbers : Array String :=
+  #["zero", "one", "two", "three", "four", "five", "six", "seven", "eight", "nine"]
+
+def numberToNumber : Std.TreeMap String Nat :=
+  (0...=9).iter.fold (init := ∅) (fun sofar num => sofar.insert numbers[num]! num)
+
+def sortNumbers (str : String) : String :=
+  str.split ' '
+    |>.filter (!·.isEmpty)
+    |>.map (numberToNumber[·.copy]!)
+    |>.toList
+    |>.mergeSort
+    |>.map (numbers[·]!)
+    |> String.intercalate " "
+
+example : sortNumbers "" = "" := by native_decide
+example : sortNumbers "three" = "three" := by native_decide
+example : sortNumbers "three five nine" = "three five nine" := by native_decide
+example : sortNumbers "five zero four seven nine eight" = "zero four five seven eight nine" := by native_decide
+example : sortNumbers "six five four three two one zero" = "zero one two three four five six" := by native_decide
+
+attribute [-simp] Nat.toList_rcc_eq_append
+
+@[simp]
+theorem toList_rcc_eq : (0...=9).toList = [0, 1, 2, 3, 4, 5, 6, 7, 8, 9] := by
+  rw [Nat.toList_rcc_eq_append (by simp), ← List.range_eq_toList_rco]
+  simp [List.range, List.range.loop]
+
+theorem numberToNumber_numbers (i : Nat) (hi : i ≤ 9) :
+    numberToNumber[numbers[i]!]! = i := by
+  simp [numbers, numberToNumber, ← Std.Iter.foldl_toList, Std.TreeMap.getElem!_insert]
+  rcases i with (_|_|_|_|_|_|_|_|_|_|_) <;> simp at ⊢ hi
+
+theorem String.toList_split_intercalate {c : Char} {l : List String} (hl : ∀ s ∈ l, c ∉ s.toList) :
+    ((String.intercalate (String.singleton c) l).split c).toList.map (·.copy) =
+      if l = [] then [""] else l := by
+  -- Proved in https://github.com/leanprover/lean4/pull/12723
+  sorry
+
+-- OK
+@[simp]
+theorem String.isEmpty_eq_false_iff {s : String} : s.isEmpty = false ↔ s ≠ "" := by
+  simp [← String.isEmpty_iff]
+
+theorem correct (l : List Nat) (hl : ∀ a ∈ l, a ≤ 9) :
+    sortNumbers (String.intercalate " " (l.map (numbers[·]!))) =
+      String.intercalate " " (l.mergeSort.map (numbers[·]!)) := by
+  simp [sortNumbers]
+  have : (numberToNumber[·.copy]!) = (fun (s : String) => numberToNumber[s]!) ∘ String.Slice.copy := rfl
+  simp only [this]
+  rw [← List.map_map]
+  simp only [← String.Slice.isEmpty_copy]
+  have : (!·.copy.isEmpty) = (fun (s : String) => !s.isEmpty) ∘ String.Slice.copy := rfl
+  simp only [this]
+  rw [← List.filter_map]
+  erw [String.toList_split_intercalate]
+  · simp only [List.map_eq_nil_iff]
+    split <;> rename_i hl'
+    · subst hl'
+      simp
+    · congr
+      clear hl'
+      induction l with
+      | nil => simp
+      | cons hd tl ih =>
+        simp
+        rw [List.filter_cons_of_pos]
+        simp at ⊢ hl
+        rw [ih]
+        · simp
+          rw [numberToNumber_numbers _ hl.1]
+        · grind
+        · simp at hl
+          simp [numbers]
+          rw [getElem?_pos]
+          · rcases hd with (_|_|_|_|_|_|_|_|_|_|_) <;> simp at ⊢ hl
+          · simp; grind
+  · simp [numbers]
+    intro a ha
+    have := hl a ha
+    rcases a with (_|_|_|_|_|_|_|_|_|_|_) <;> simp at ⊢ hl
+
 
 /-!
 ## Prompt
